Added definition of VSU.LinkedProgVSU and modified proof of link_pile.pile_correct.

progs/VSUpile/link_pile.v
@@ -7,58 +7,25 @@ Import main.
 Notation LinkCanonicalComponent1 := MainComponent_with_ExtsInE.LinkCanonicalComponent1.
 Notation Gprog:= MainComponent_with_ExtsInE.Gprog.
 Notation Vprog:= MainComponent_with_ExtsInE.Vprog.
-Notation Imports:= MainComponent_with_ExtsInE.Imports.
-Notation G:= MainComponent_with_ExtsInE.G.
+
+Definition Exports := [main_spec linked_prog].
 
 (*Succeeds as imports are now empty*)
 Definition APPLIC:= @Canonical_semaxfunc _ _ _ _ _ _ _ LinkCanonicalComponent1.
+(*Definition is dead, but the reminder Imports empty is important*)
 
-Definition AGG_pre := augment_funspecs linked_prog Gprog.
+Notation PileMainVSU := MainComponent_with_ExtsInE.PileVSU.
 
-  Definition AGG := ltac:
-  (let x := eval hnf in AGG_pre in
-   let x := eval simpl in x in 
-   (*let x := eval compute in x in *)
-       exact x).
-
-Lemma AGG_char i: find_id i (augment_funspecs linked_prog Gprog) = find_id i AGG.
+Lemma prog_correct:
+  exists G, 
+ @semax_prog NullExtension.Espec LinkedCompSpecs linked_prog tt Vprog G(*prog*).
 Proof.
-remember (find_id i AGG) as d; symmetry in Heqd. destruct d.
-+ assert (X:= find_id_In_map_fst _ _ _ Heqd). cbv in X.
-  repeat (destruct X as [Hi | X]; [ subst i; apply Heqd |]).
-  contradiction.
-+ remember (find_id i (augment_funspecs linked_prog Gprog)) as e; symmetry in Heqe; destruct e; trivial.
-  assert (X:= find_id_In_map_fst _ _ _ Heqe). cbv in X.
-  repeat (destruct X as [Hi | X]; [ subst i; inv Heqd |]).
-  contradiction.
-Qed.
-(*
-Axiom ExternalInfo_funspec_sub: forall {Espec ge i e ts t c phi}
-(SFE: semaxfunc_ExternalInfo Espec ge i e ts t c phi)
-(phi' : funspec)
-(Fsub : funspec_sub phi phi'),
-semaxfunc_ExternalInfo Espec ge i e ts t c phi'.
-(*NOT provable currently -- see VSU*)
-
-Lemma semaxfunc_funspec_sub {Espec cs V G ge}: forall funs G1 G2,
-@semaxfunc Espec cs V G ge funs G1 ->
-Forall2 (fun fs1 fs2 => fst fs1 = fst fs2 /\ funspec_sub (snd fs1) (snd fs2)) G1 G2 ->
-@semaxfunc Espec cs V G ge funs G2.
-Proof. induction funs; intros; inv H; inv H0. constructor.
-+ destruct y as [i psi]. simpl in H2. destruct H2; subst.
-  constructor; trivial.
-  eapply InternalInfo_funspec_sub; eassumption.
-  eauto.
-+ destruct y as [i psi]. simpl in H2. destruct H2; subst.
-  constructor; trivial.
-  eapply ExternalInfo_funspec_sub; eassumption.
-  eauto.
-Qed.*)
-
-Lemma prog_correct: 
- @semax_prog NullExtension.Espec LinkedCompSpecs linked_prog tt Vprog Gprog.
-Proof.
-(*  prove_semax_prog.*)
+  destruct PileMainVSU as [G [Comp MAIN]]. exists G.
+  assert (DomG: map fst G = map fst (prog_funct linked_prog)).
+  { destruct Comp. unfold Comp_G in *. rewrite CC_canonical.
+    cbv; reflexivity. }
+(*  specialize (Comp_G_Exports Comp _main _ (eq_refl _)); intros.*)
+(*  prove_semax_prog. failes*)
 (*Ltac prove_semax_prog_aux tac :=*)
   (*match goal with
     | |- semax_prog ?prog ?z ?Vprog ?Gprog =>
@@ -80,10 +47,8 @@ Proof.
         fail "Funspec of _main is not in the proper form")
     end*)
  ].
-  all: rewrite augment_funspecs_eq by reflexivity.
-  2:{ assert (prog_main linked_prog = _main) by reflexivity. rewrite H.
-      (*rewrite AGG_char.*)
-      simpl. eexists; try (unfold NDmk_funspec'; rewrite_old_main_pre); reflexivity. }
+  all: rewrite augment_funspecs_eq by trivial.
+  2:{ destruct MAIN as [post [ora MAIN]]. rewrite MAIN. exists post. destruct ora. trivial.  }
  (*
  match goal with |- semax_func ?V ?G ?g ?D ?G' =>
    let Gprog := fresh "Gprog" in 
@@ -92,8 +57,9 @@ Proof.
  end.
  tac.*)
 (*finish_semax_prog. *)
-specialize APPLIC; intros APP.
-(*eapply (semaxfunc_funspec_sub _ _ (augment_funspecs linked_prog Gprog)) in APP.*)
+apply (@Canonical_semax_func _ _ _ _ _ _ _ Comp). cbv; reflexivity.
+(*OLD PROOF
+specialize (@Canonical_semaxfunc _ _ _ _ _ _ _ LinkCanonicalComponent1); intros APP.
 + apply semaxfunc_sound in APP.
   assert (HG: Comp_G LinkCanonicalComponent1 = Gprog) by reflexivity. unfold Imports in HG.
   rewrite filter_true in APP. 
@@ -107,5 +73,5 @@ specialize APPLIC; intros APP.
       rewrite HH. intros. apply sub_option_refl.
   - clear APP; intros [i fd] Hi. cbv in Hi.
     repeat ( destruct Hi as [X | Hi]; [ inv X; reflexivity |] ).
-    contradiction.
+    contradiction.*)
 Qed.
